spi_model/SPI_tauScript.sml
@@ -31,7 +31,7 @@ state := init_setregs (* enter the next init state, set up SPI registers *) |>`
 val tx_channel_enabled_op_def = Define `
 tx_channel_enabled_op (spi:spi_state) =
 spi with <|regs := spi.regs with CH0STAT := spi.regs.CH0STAT 
-with <|TXS := 1w; EOT := 0w |>;
+with TXS := 1w;
 state := tx_ready_for_trans |>`
 
 (* SPI controller's operation after TX0 register was set. 
@@ -74,7 +74,7 @@ state := rx_data_ready |>`
 val xfer_channel_enabled_op_def = Define `
 xfer_channel_enabled_op (spi:spi_state) = 
 spi with <| regs := spi.regs with CH0STAT := spi.regs.CH0STAT
-with <|RXS := 0w; TXS := 1w; EOT := 1w |>;
+with <|RXS := 0w; TXS := 1w |>;
 state := xfer_ready_for_trans |>`
 
 (* Update theTX_SHIFT_REG after TX0 was written.
