spi_model/SPI_update_regsScript.sml
@@ -232,7 +232,7 @@ val write_TX0_def = Define `
 write_TX0 (value:word32) (spi:spi_state) =
 let wl = (w2n spi.regs.CH0CONF.WL) in
 if (CHECK_TXS_BIT spi) /\ (spi.state = tx_ready_for_trans) then
-spi with <| regs := spi.regs with <| CH0STAT := spi.regs.CH0STAT with TXS := 0w;
+spi with <| regs := spi.regs with <| CH0STAT := spi.regs.CH0STAT with <| TXS := 0w; EOT := 0w |>;
 TX0 := ((wl >< 0) value:word32) |>;
 state := tx_trans_data |>
 else if (CHECK_TXS_BIT spi) /\ (spi.state = xfer_ready_for_trans) then
