thm/abs1_comb_hold_ref_rel_RD_REScript.sml
@@ -1,4 +1,5 @@
 open HolKernel bossLib boolLib Parse;
+open wordsLib pred_setLib;
 open SPI_stateTheory SPI_relationTheory SPI_return_regsTheory;
 open driver_stateTheory driver_relationTheory driver_readTheory;
 open ds_abs1_stateTheory ds_abs1_relTheory ds_abs1_initTheory ds_abs1_txTheory 
@@ -7,24 +8,255 @@ open ref_relTheory board_memTheory;
 
 val _ = new_theory "abs1_comb_hold_ref_rel_RD_RE";
 
+(* relation holds when driver state is dr_init_read_req *)
 val ref_rel_hold_dr_init_read_req = store_thm("ref_rel_hold_dr_init_read_req",
 ``!(spi:spi_state) (dr:driver_state) (ds_abs1:ds_abs1_state).
 (ref_rel ds_abs1 dr spi) /\ (dr.state = dr_init_read_req) /\
 (spi_tr spi (Return (THE (dr_read dr).dr_last_read_ad) v) spi') ==>
 ref_rel ds_abs1 (dr_read dr with dr_last_read_v := SOME v) spi'``,
 rw [spi_tr_cases, dr_read_def, dr_read_sysstatus_def, read_SPI_regs_state_def,
-read_SPI_regs_value_def, read_SPI_regs_def] >>
-cheat);
+read_SPI_regs_value_def] >>
+rw [read_SPI_regs_def] >|
+[FULL_SIMP_TAC (std_ss++WORD_ss++PRED_SET_ss) 
+[SPI0_SYSSTATUS_def, SPI0_PA_RANGE_def, SPI0_START_def, SPI0_END_def],
+FULL_SIMP_TAC (std_ss++WORD_ss) [SPI0_SYSSTATUS_def, SPI0_SYSCONFIG_def],
+FULL_SIMP_TAC std_ss [ref_rel_def, IS_STATE_REL_def] >>
+rw []]);
 
+(* relation holds when driver state is dr_tx_read_txs *)
+val ref_rel_hold_dr_tx_read_txs = store_thm("ref_rel_hold_dr_tx_read_txs",
+``!(spi:spi_state) (dr:driver_state) (ds_abs1:ds_abs1_state).
+(ref_rel ds_abs1 dr spi) /\ (dr.state = dr_tx_read_txs) /\
+(spi_tr spi (Return (THE (dr_read dr).dr_last_read_ad) v) spi') ==>
+ref_rel ds_abs1 (dr_read dr with dr_last_read_v := SOME v) spi'``,
+rw [spi_tr_cases, dr_read_def, dr_read_ch0stat_def, read_SPI_regs_state_def,
+read_SPI_regs_value_def] >>
+rw [read_SPI_regs_def, SPI0_CH0STAT_def, SPI0_PA_RANGE_def, SPI0_START_def,
+SPI0_END_def, SPI0_SYSCONFIG_def, SPI0_SYSSTATUS_def, SPI0_MODULCTRL_def,
+SPI0_CH0CONF_def] >>
+FULL_SIMP_TAC std_ss [ref_rel_def, IS_STATE_REL_def] >>
+rw [SPI0_CH0STAT_def, build_CH0STAT_def] >>
+FULL_SIMP_TAC (std_ss++WORD_BIT_EQ_ss) []);
 
-(* simulation: ds_abs1' exists and holds the ref_rel when driver_tau *)
+(* relation holds when driver state is dr_tx_read_eot *)
+val ref_rel_hold_dr_tx_read_eot = store_thm("ref_rel_hold_dr_tx_read_eot",
+``!(spi:spi_state) (dr:driver_state) (ds_abs1:ds_abs1_state).
+(ref_rel ds_abs1 dr spi) /\ (dr.state = dr_tx_read_eot) /\
+(spi_tr spi (Return (THE (dr_read dr).dr_last_read_ad) v) spi') ==>
+ref_rel ds_abs1 (dr_read dr with dr_last_read_v := SOME v) spi'``,
+rw [spi_tr_cases, dr_read_def, dr_read_ch0stat_def, read_SPI_regs_state_def,
+read_SPI_regs_value_def] >>
+rw [read_SPI_regs_def, SPI0_CH0STAT_def, SPI0_PA_RANGE_def, SPI0_START_def,
+SPI0_END_def, SPI0_SYSCONFIG_def, SPI0_SYSSTATUS_def, SPI0_MODULCTRL_def,
+SPI0_CH0CONF_def] >>
+FULL_SIMP_TAC std_ss [ref_rel_def, IS_STATE_REL_def] >>
+rw [SPI0_CH0STAT_def, build_CH0STAT_def] >>
+FULL_SIMP_TAC (std_ss++WORD_BIT_EQ_ss) []);
+
+(* relation holds when driver state is dr_rx_read_rxs *)
+val ref_rel_hold_dr_rx_read_rxs = store_thm("ref_rel_hold_dr_rx_read_rxs",
+``!(spi:spi_state) (dr:driver_state) (ds_abs1:ds_abs1_state).
+(ref_rel ds_abs1 dr spi) /\ (dr.state = dr_rx_read_rxs) /\
+(spi_tr spi (Return (THE (dr_read dr).dr_last_read_ad) v) spi') ==>
+ref_rel ds_abs1 (dr_read dr with dr_last_read_v := SOME v) spi'``,
+rw [spi_tr_cases, dr_read_def, dr_read_ch0stat_def, read_SPI_regs_state_def,
+read_SPI_regs_value_def] >>
+rw [read_SPI_regs_def, SPI0_CH0STAT_def, SPI0_PA_RANGE_def, SPI0_START_def,
+SPI0_END_def, SPI0_SYSCONFIG_def, SPI0_SYSSTATUS_def, SPI0_MODULCTRL_def,
+SPI0_CH0CONF_def] >>
+FULL_SIMP_TAC std_ss [ref_rel_def, IS_STATE_REL_def] >>
+rw [SPI0_CH0STAT_def, build_CH0STAT_def] >>
+FULL_SIMP_TAC (std_ss++WORD_BIT_EQ_ss) []);
+
+(* lemma: if dr.state = dr_rx_read_rx0 then ds_abs1.state = abs1_rx_ready
+   according to ref_rel *)
+val dr_rx_read_rx0_imply_abs1_rx_ready = 
+store_thm("dr_rx_read_rx0_imply_abs1_rx_ready",
+``!(spi:spi_state) (dr:driver_state) (ds_abs1:ds_abs1_state).
+(ref_rel ds_abs1 dr spi) /\ (dr.state = dr_rx_read_rx0) ==>
+ds_abs1.state = abs1_rx_ready``,
+rw [] >>
+`IS_STATE_REL ds_abs1 dr spi` by METIS_TAC [ref_rel_def] >>
+FULL_SIMP_TAC std_ss [IS_STATE_REL_def] >>
+Cases_on `spi.state` >>
+rw [] >>
+`(dr.state <> dr_init_pre) /\
+(dr.state <> dr_init_idle) /\
+(dr.state <> dr_init_read_req) /\
+(dr.state <> dr_init_check_rep) /\
+(dr.state <> dr_init_setting) /\
+(dr.state <> dr_ready) /\
+(dr.state <> dr_tx_idle) /\
+(dr.state <> dr_tx_conf_issued) /\
+(dr.state <> dr_tx_read_txs) /\
+(dr.state <> dr_tx_check_txs) /\
+(dr.state <> dr_tx_write_data) /\
+(dr.state <> dr_tx_read_eot) /\
+(dr.state <> dr_tx_check_eot) /\
+(dr.state <> dr_tx_issue_disable) /\
+(dr.state <> dr_tx_reset_conf) /\
+(dr.state <> dr_rx_idle) /\
+(dr.state <> dr_rx_conf_issued) /\
+(dr.state <> dr_rx_read_rxs) /\
+(dr.state <> dr_rx_check_rxs) /\
+(dr.state <> dr_rx_fetch_data) /\
+(dr.state <> dr_rx_issue_disable) /\
+(dr.state <> dr_rx_reset_conf) /\
+(dr.state <> dr_xfer_idle) /\
+(dr.state <> dr_xfer_conf_issued) /\
+(dr.state <> dr_xfer_read_txs) /\
+(dr.state <> dr_xfer_check_txs) /\
+(dr.state <> dr_xfer_write_dataO) /\
+(dr.state <> dr_xfer_read_rxs) /\
+(dr.state <> dr_xfer_check_rxs) /\
+(dr.state <> dr_xfer_read_rx0) /\
+(dr.state <> dr_xfer_fetch_dataI) /\
+(dr.state <> dr_xfer_issue_disable) /\
+(dr.state <> dr_xfer_reset_conf)` by rw [] >>
+Cases_on `ds_abs1.state` >>
+rw []);
+
+(* ds_abs1' exists and relation holds when driver state is dr_rx_read_rx0 *)
+val ref_rel_hold_dr_rx_read_rx0 = store_thm("ref_rel_hold_dr_rx_read_rx0",
+``!(spi:spi_state) (dr:driver_state) (ds_abs1:ds_abs1_state).
+(ref_rel ds_abs1 dr spi) /\ (dr.state = dr_rx_read_rx0) /\
+(spi_tr spi (Return (THE (dr_read dr).dr_last_read_ad) v) spi') ==>
+?ds_abs1'.(ds_abs1_tr ds_abs1 tau ds_abs1') /\
+(ref_rel ds_abs1' (dr_read dr with dr_last_read_v := SOME v) spi')``,
+rw [spi_tr_cases, dr_read_def, dr_read_rx0_def, read_SPI_regs_state_def,
+read_SPI_regs_value_def, ds_abs1_tr_cases, ds_abs1_comb_tr_cases] >>
+`ds_abs1.state = abs1_rx_ready` by METIS_TAC [dr_rx_read_rx0_imply_abs1_rx_ready] >>
+`spi.state = rx_data_ready` by METIS_TAC [ref_rel_def, IS_STATE_REL_def] >>
+EXISTS_TAC ``comb_abs1_rx_operations ds_abs1`` >>
+rw [COMB_ABS1_RX_ENABLE_def, read_SPI_regs_def, SPI0_RX0_def, SPI0_PA_RANGE_def, 
+SPI0_START_def, SPI0_END_def, SPI0_SYSCONFIG_def, SPI0_SYSSTATUS_def, 
+SPI0_MODULCTRL_def, SPI0_CH0CONF_def, SPI0_CH0STAT_def, SPI0_CH0CTRL_def,
+SPI0_TX0_def, SPI0_RX0_def, comb_abs1_rx_operations_def, 
+comb_abs1_rx_ready_op_def, read_RX0_def] >|
+[FULL_SIMP_TAC std_ss [ref_rel_def, IS_STATE_REL_def] >>
+rw [SPI0_RX0_def] >>
+Cases_on `dr.state` >>
+rw [] >>
+FULL_SIMP_TAC (std_ss++WORD_BIT_EQ_ss) [],
+FULL_SIMP_TAC std_ss [ref_rel_def, CHECK_RXS_BIT_def]]);
+
+(* relation holds when driver state is dr_xfer_read_txs *)
+val ref_rel_hold_dr_xfer_read_txs = store_thm("ref_rel_hold_dr_xfer_read_txs",
+``!(spi:spi_state) (dr:driver_state) (ds_abs1:ds_abs1_state).
+(ref_rel ds_abs1 dr spi) /\ (dr.state = dr_xfer_read_txs) /\
+(spi_tr spi (Return (THE (dr_read dr).dr_last_read_ad) v) spi') ==>
+ref_rel ds_abs1 (dr_read dr with dr_last_read_v := SOME v) spi'``,
+rw [spi_tr_cases, dr_read_def, dr_read_ch0stat_def, read_SPI_regs_state_def,
+read_SPI_regs_value_def] >>
+rw [read_SPI_regs_def, SPI0_CH0STAT_def, SPI0_PA_RANGE_def, SPI0_START_def,
+SPI0_END_def, SPI0_SYSCONFIG_def, SPI0_SYSSTATUS_def, SPI0_MODULCTRL_def,
+SPI0_CH0CONF_def] >>
+FULL_SIMP_TAC std_ss [ref_rel_def, IS_STATE_REL_def] >>
+rw [SPI0_CH0STAT_def, build_CH0STAT_def] >>
+FULL_SIMP_TAC (std_ss++WORD_BIT_EQ_ss) []);
+
+(* relation holds when driver state is dr_xfer_read_rxs *)
+val ref_rel_hold_dr_xfer_read_rxs = store_thm("ref_rel_hold_dr_xfer_read_rxs",
+``!(spi:spi_state) (dr:driver_state) (ds_abs1:ds_abs1_state).
+(ref_rel ds_abs1 dr spi) /\ (dr.state = dr_xfer_read_rxs) /\
+(spi_tr spi (Return (THE (dr_read dr).dr_last_read_ad) v) spi') ==>
+ref_rel ds_abs1 (dr_read dr with dr_last_read_v := SOME v) spi'``,
+rw [spi_tr_cases, dr_read_def, dr_read_ch0stat_def, read_SPI_regs_state_def,
+read_SPI_regs_value_def] >>
+rw [read_SPI_regs_def, SPI0_CH0STAT_def, SPI0_PA_RANGE_def, SPI0_START_def,
+SPI0_END_def, SPI0_SYSCONFIG_def, SPI0_SYSSTATUS_def, SPI0_MODULCTRL_def,
+SPI0_CH0CONF_def] >>
+FULL_SIMP_TAC std_ss [ref_rel_def, IS_STATE_REL_def] >>
+rw [SPI0_CH0STAT_def, build_CH0STAT_def] >>
+FULL_SIMP_TAC (std_ss++WORD_BIT_EQ_ss) []);
+
+(* lemma: if dr.state = dr_xfer_read_rx0, then ds_abs1.state = abs1_xfer_ready 
+   according to the ref_rel *)
+val dr_xfer_read_rx0_imply_abs1_xfer_ready = 
+store_thm("dr_xfer_read_rx0_imply_abs1_xfer_ready",
+``!(spi:spi_state) (dr:driver_state) (ds_abs1:ds_abs1_state).
+(ref_rel ds_abs1 dr spi) /\ (dr.state = dr_xfer_read_rx0) ==>
+ds_abs1.state = abs1_xfer_ready``,
+rw [] >>
+`IS_STATE_REL ds_abs1 dr spi` by METIS_TAC [ref_rel_def] >>
+FULL_SIMP_TAC std_ss [IS_STATE_REL_def] >>
+Cases_on `spi.state` >>
+rw [] >>
+`(dr.state <> dr_init_pre) /\
+(dr.state <> dr_init_idle) /\
+(dr.state <> dr_init_read_req) /\
+(dr.state <> dr_init_check_rep) /\
+(dr.state <> dr_init_setting) /\
+(dr.state <> dr_ready) /\
+(dr.state <> dr_tx_idle) /\
+(dr.state <> dr_tx_conf_issued) /\
+(dr.state <> dr_tx_read_txs) /\
+(dr.state <> dr_tx_check_txs) /\
+(dr.state <> dr_tx_write_data) /\
+(dr.state <> dr_tx_read_eot) /\
+(dr.state <> dr_tx_check_eot) /\
+(dr.state <> dr_tx_issue_disable) /\
+(dr.state <> dr_tx_reset_conf) /\
+(dr.state <> dr_rx_idle) /\
+(dr.state <> dr_rx_conf_issued) /\
+(dr.state <> dr_rx_read_rxs) /\
+(dr.state <> dr_rx_check_rxs) /\
+(dr.state <> dr_rx_read_rx0) /\
+(dr.state <> dr_rx_fetch_data) /\
+(dr.state <> dr_rx_issue_disable) /\
+(dr.state <> dr_rx_reset_conf) /\
+(dr.state <> dr_xfer_idle) /\
+(dr.state <> dr_xfer_conf_issued) /\
+(dr.state <> dr_xfer_read_txs) /\
+(dr.state <> dr_xfer_check_txs) /\
+(dr.state <> dr_xfer_write_dataO) /\
+(dr.state <> dr_xfer_read_rxs) /\
+(dr.state <> dr_xfer_check_rxs) /\
+(dr.state <> dr_xfer_fetch_dataI) /\
+(dr.state <> dr_xfer_issue_disable) /\
+(dr.state <> dr_xfer_reset_conf)` by rw [] >>
+Cases_on `ds_abs1.state` >>
+rw []);
+
+(* ds_abs1' exists and relation holds when driver state is dr_xfer_read_rx0 *)
+val ref_rel_hold_dr_xfer_read_rx0 = store_thm("ref_rel_hold_dr_xfer_read_rx0",
+``!(spi:spi_state) (dr:driver_state) (ds_abs1:ds_abs1_state).
+(ref_rel ds_abs1 dr spi) /\ (dr.state = dr_xfer_read_rx0) /\
+(spi_tr spi (Return (THE (dr_read dr).dr_last_read_ad) v) spi') ==>
+?ds_abs1'.(ds_abs1_tr ds_abs1 tau ds_abs1') /\
+(ref_rel ds_abs1' (dr_read dr with dr_last_read_v := SOME v) spi')``,
+rw [spi_tr_cases, dr_read_def, dr_read_rx0_def, read_SPI_regs_state_def,
+read_SPI_regs_value_def, ds_abs1_tr_cases, ds_abs1_comb_tr_cases] >>
+`ds_abs1.state = abs1_xfer_ready` by METIS_TAC [dr_xfer_read_rx0_imply_abs1_xfer_ready] >>
+`spi.state = xfer_data_ready` by METIS_TAC [ref_rel_def, IS_STATE_REL_def] >>
+EXISTS_TAC ``comb_abs1_xfer_operations ds_abs1`` >>
+rw [COMB_ABS1_XFER_ENABLE_def, read_SPI_regs_def, SPI0_RX0_def, SPI0_PA_RANGE_def, 
+SPI0_START_def, SPI0_END_def, SPI0_SYSCONFIG_def, SPI0_SYSSTATUS_def, 
+SPI0_MODULCTRL_def, SPI0_CH0CONF_def, SPI0_CH0STAT_def, SPI0_CH0CTRL_def,
+SPI0_TX0_def, SPI0_RX0_def, comb_abs1_xfer_operations_def, 
+comb_abs1_xfer_ready_op_def, read_RX0_def] >|
+[FULL_SIMP_TAC std_ss [ref_rel_def, IS_STATE_REL_def] >>
+rw [SPI0_RX0_def] >>
+Cases_on `dr.state` >>
+rw [] >>
+FULL_SIMP_TAC (std_ss++WORD_BIT_EQ_ss) [],
+FULL_SIMP_TAC std_ss [ref_rel_def, CHECK_RXS_BIT_def]]);
+
+(* simulation: ref_rel holds for ds_abs1 or ds_abs1' when driver and controller perform read and return operations *)
 val abs1_comb_hold_ref_rel_RD_RE = store_thm("abs1_comb_hold_ref_rel_RD_RE",
 ``!(spi:spi_state) (dr:driver_state) (ds_abs1:ds_abs1_state).
 (ref_rel ds_abs1 dr spi) /\ (driver_tr dr (Read a v) dr') /\ 
 (spi_tr spi (Return a v) spi') ==>
 (ref_rel ds_abs1 dr' spi') \/
 (?ds_abs1'.(ds_abs1_tr ds_abs1 tau ds_abs1') /\ (ref_rel ds_abs1' dr' spi'))``,
-rw [driver_tr_cases, DR_RD_ENABLE_def] >>
-cheat);
+rw [driver_tr_cases, DR_RD_ENABLE_def] >|
+[METIS_TAC [ref_rel_hold_dr_init_read_req],
+METIS_TAC [ref_rel_hold_dr_tx_read_txs],
+METIS_TAC [ref_rel_hold_dr_tx_read_eot],
+METIS_TAC [ref_rel_hold_dr_rx_read_rxs],
+METIS_TAC [ref_rel_hold_dr_rx_read_rx0],
+METIS_TAC [ref_rel_hold_dr_xfer_read_txs],
+METIS_TAC [ref_rel_hold_dr_xfer_read_rxs],
+METIS_TAC [ref_rel_hold_dr_xfer_read_rx0]]);
 
 val _ = export_theory();
